BICONDITIONAL ELIMINATION is the name of two valid rules of inference of propositional logic. It allows for one to infer a conditional from a biconditional. If P ↔ Q is true, then one may infer that P → Q is true, and also that Q → P is true.[1] For example, if it's true that I'm breathing if and only if I'm alive, then it's true that if I'm breathing, I'm alive; likewise, it's true that if I'm alive, I'm breathing. The rules can be stated formally as:

$$\frac{P \leftrightarrow Q}{\therefore P \to Q}$$
and

$$\frac{P \leftrightarrow Q}{\therefore Q \to P}$$

where the rule is that wherever an instance of "P ↔ Q" appears on a line of a proof, either "P → Q" or "Q → P" can be placed on a subsequent line;


Formal notation

The _biconditional elimination_ rule may be written in sequent notation:

(_P_ ↔ _Q_) ⊢ (_P_ → _Q_)
and

(_P_ ↔ _Q_) ⊢ (_Q_ → _P_)

where ⊢ is a metalogical symbol meaning that P → Q, in the first case, and Q → P in the other are syntactic consequences of P ↔ Q in some logical system;

or as the statement of a truth-functional tautology or theorem of propositional logic:

(_P_ ↔ _Q_) → (_P_ → _Q_)

(_P_ ↔ _Q_) → (_Q_ → _P_)

where P, and Q are propositions expressed in some formal system.


See also

-   Logical biconditional


References

Category:Rules of inference Category:Theorems in propositional logic

[1]